Trasportata prima parte definizioni da proofs a file base

MasterThesis/Compiler/Compiler_v2.lean
@@ -1,10 +1,23 @@
+/-
+"A Lean-certified reversibilization of Meyer-Ritchie LOOP language".
+Master thesis in computer science, University of Turin.
+Authors: Andrea Delmastro
+-/
 import MasterThesis.SCORE.Language
 import MasterThesis.LOOP.Language
+
+/-!
+# Compiler for LOOP language, version 2
+-/
+
+namespace Compiler
 
 open LOOP Com
 open SCORE Com
 
-def l2s' (ev : Ident) (P : LOOP.Com) : SCORE.Com :=
+namespace v2
+
+def l2s (ev : Ident) (P : LOOP.Com) : SCORE.Com :=
   CON ev;;
   match P with
   | .SKIP     => SKIP
@@ -14,6 +27,21 @@ def l2s' (ev : Ident) (P : LOOP.Com) : SCORE.Com :=
                  FOR ev (INC x);;
                  FOR x (DEC ev)
   | .INC x    => INC x
-  | .SEQ P Q  => l2s' ev P;;
-                 l2s' ev Q
-  | .LOOP x P => FOR x (l2s' ev P)
+  | .SEQ P Q  => l2s ev P;;
+                 l2s ev Q
+  | .LOOP x P => FOR x (l2s ev P)
+
+end v2
+
+open v2
+
+def eq_states_idents (s : LOOP.State) (t : SCORE.State) (ids : Finset Ident) : Prop :=
+  match s, t with
+  | some σ, some τ => ∀ (x : Ident), x ∈ ids → some ↑(σ x) = (τ x).head?
+  | _     , _      => False
+
+notation:50 s:50 "∼[" P:50 "]" t:50 => eq_states_idents s t P
+
+lemma eq_states_idents_subs {s : LOOP.State} {t : SCORE.State} {a b : Finset Ident} : s ∼[a ∪ b] t → s ∼[a] t := by sorry
+
+end Compiler
