MasterThesis/Compiler/Proofs/Commons.lean
@@ -1,6 +1,0 @@
-import Mathlib.Tactic.Basic
-import MasterThesis.LOOP.Language
-import MasterThesis.SCORE.Language
-import MasterThesis.Compiler.Commons
-
-lemma eq_states_idents_subs {s : LOOP.State} {t : SCORE.State} {a b : Finset Ident} : s =[a ∪ b]ₛ t → s =[a]ₛ t := by sorry
